formal-proofs/theories/lib/interruptible_semaphore/interruptible_semaphore.v
@@ -1,0 +1,135 @@
+From iris.heap_lang Require Import notation.
+
+Require Import SegmentQueue.lib.thread_queue.thread_queue.
+
+Section impl.
+
+Variable segment_size : positive.
+
+Definition new_semaphore : val :=
+  λ: "n", "availablePermits" <- ref "n" ;;
+          ("availablePermits", new_thread_queue segment_size #()).
+
+Definition cancellation_handler : val :=
+  λ: "availablePermits" "head" "deqIdx" "canceller",
+  let: "p" := FAA "availablePermits" #1
+  in if: #0 ≤ "p" then #() else
+  if: "canceller" #() then #()
+  else resume segment_size "head" "deqIdx".
+
+Definition acquire_semaphore : val :=
+  λ: "cancHandle" "threadHandle" "availablePermits" "tail" "enqIdx" "head" "deqIdx",
+  let: "p" := FAA "availablePermits"  #(-1)
+  in if: #0 < "p" then #()
+  else suspend segment_size
+               (cancellation_handler "availablePermits" "head" "deqIdx")
+               "threadHandle" "tail" "enqIdx".
+
+Definition release_semaphore : val :=
+  λ: "availablePermits" "head" "deqIdx",
+  let: "p" := FAA "availablePermits" #1
+  in if: #0 ≤ "p" then #()
+  else resume segment_size "head" "deqIdx".
+
+End impl.
+
+From iris.heap_lang Require Import proofmode.
+From iris.algebra Require Import auth.
+From iris.algebra Require Import list gset excl csum.
+From iris.program_logic Require Import atomic.
+
+Require Import SegmentQueue.lib.infinite_array.infinite_array_impl.
+Require Import SegmentQueue.lib.infinite_array.iterator.
+
+Section proof.
+
+Notation algebra := (authR (prodUR natUR natUR)).
+
+Class semaphoreG Σ := SemaphoreG { semaphore_inG :> inG Σ algebra }.
+Definition semaphoreΣ : gFunctors := #[GFunctor algebra].
+Instance subG_semaphoreΣ {Σ} : subG semaphoreΣ Σ -> semaphoreG Σ.
+Proof. solve_inG. Qed.
+
+Context `{iArrayG Σ} `{iteratorG Σ} `{heapG Σ} `{threadQueueG Σ} `{semaphoreG Σ} `{parkingG Σ}.
+Variable (N: namespace).
+Notation iProp := (iProp Σ).
+
+Variable (segment_size: positive).
+
+Definition is_semaphore (R : iProp) (γ: gname) (availablePermits: nat) (p: loc)
+  (epℓ eℓ dpℓ dℓ: loc) (γa γtq γe γd: gname) :=
+  (∃ (readyToCancel: nat) l deqFront,
+  ([∗ list] _ ∈ seq 0 availablePermits, R) ∗
+   own γ (● (availablePermits, readyToCancel)) ∗
+   is_thread_queue N segment_size True R γa γtq γe γd eℓ epℓ dℓ dpℓ l deqFront ∗
+   let v := count_matching still_present (drop deqFront l) in
+   p ↦ #(availablePermits - v + readyToCancel) ∗
+   ⌜readyToCancel <= v ∧ (availablePermits = 0 ∨ v = readyToCancel)%nat⌝)%I.
+
+Theorem release_semaphore_spec R γ (p epℓ eℓ dpℓ dℓ: loc) γa γtq γe γd:
+  R -∗
+  <<< ∀ availablePermits, is_semaphore R γ availablePermits p epℓ eℓ dpℓ dℓ γa γtq γe γd >>>
+    (release_semaphore segment_size) #p #dℓ #dpℓ @ ⊤
+  <<< is_semaphore R γ (1 + availablePermits)%nat p epℓ eℓ dpℓ dℓ γa γtq γe γd, RET #() >>>.
+Proof.
+  iIntros "HR" (Φ) "AU". wp_lam. wp_pures.
+  wp_bind (FAA _ _).
+  iMod "AU" as (availablePermits) "[HIsSem HClose]".
+  iDestruct "HIsSem" as (readyToCancel l deqFront) "(HPerms & HAuth & HTq & Hp & HPure)".
+  iDestruct "HPure" as %HPure.
+  remember (count_matching _ _) as v.
+  remember (availablePermits - v + readyToCancel) as op.
+  wp_faa.
+  destruct (decide (0 <= op)).
+  {
+    iDestruct "HClose" as "[_ HClose]".
+    iMod (own_update with "HAuth") as "[HAuth HFrag]".
+    {
+      apply auth_update_alloc.
+      apply prod_local_update_1.
+      apply (nat_local_update availablePermits 0%nat _ 1%nat).
+      auto.
+    }
+    repeat rewrite Nat.add_1_r.
+    iMod ("HClose" with "[-]") as "HΦ".
+    {
+      iExists _, _, _. simpl. iFrame "HR HAuth HTq".
+      iSplitL "HPerms".
+      {
+        iApply (big_opL_forall' with "HPerms").
+        by repeat rewrite seq_length.
+        done.
+      }
+      iSplitL.
+      {
+        rewrite -Heqv Heqop.
+        replace (S availablePermits - v + readyToCancel)
+                with (availablePermits - v + readyToCancel + 1).
+        done.
+        lia.
+      }
+      iPureIntro.
+      split; lia.
+    }
+    iModIntro. wp_pures. rewrite bool_decide_decide.
+    destruct (decide (0 <= op)); try lia. by wp_pures.
+  }
+
+  assert (v > 0) as HExistsNondequed by lia.
+  move: HExistsNondequed. subst; clear. move=> HExistsNondequed.
+
+  iDestruct "HTq" as "(HInfArr & HListContents & HRest)".
+  iDestruct (cell_list_contents_register_for_dequeue
+               with "HR HListContents") as ">[[HAwak HDeqFront] [HListContents _]]".
+  {
+    admit.
+  }
+
+  iDestruct "HClose" as "[HClose _]".
+  iMod ("HClose" with "[-HDeqFront HAwak]") as "HΦ".
+  {
+    iExists _, _, _. iFrame "HAuth HPerms HInfArr".
+
+Abort.
+
+End proof.
